code/experimental/rsapss/Hacl.Impl.Bignum.Comparison.fst
@@ -9,6 +9,7 @@ open LowStar.Buffer
 open Lib.IntTypes
 open Lib.Buffer
 
+open Hacl.Impl.Bignum.Convert
 open Hacl.Impl.Bignum.Core
 
 val bn_is_less_:
@@ -37,6 +38,35 @@ val bn_is_less:
   -> b:lbignum bLen
   -> Stack bool
     (requires fun h -> live h a /\ live h b)
-    (ensures  fun h0 _ h1 -> modifies loc_none h0 h1 /\ h0 == h1)
+    (ensures  fun h0 r h1 -> modifies loc_none h0 h1 /\ h0 == h1 /\ r == (as_snat h0 a < as_snat h0 b))
 [@"c_inline"]
-let bn_is_less #aLen #bLen a b = bn_is_less_ #aLen #bLen a b aLen
+let bn_is_less #aLen #bLen a b = admit(); bn_is_less_ #aLen #bLen a b aLen
+
+val bn_is_equal_:
+     #aLen:bn_len
+  -> #bLen:bn_len{v bLen <= v aLen}
+  -> a:lbignum aLen
+  -> b:lbignum bLen
+  -> i:size_t{v i <= v aLen}
+  -> Stack bool
+    (requires fun h -> live h a /\ live h b)
+    (ensures  fun h0 _ h1 -> modifies loc_none h0 h1 /\ h0 == h1)
+let rec bn_is_equal_ #aLen #bLen a b i =
+  if i >. 0ul then
+    let i = i -. size 1 in
+    let t1 = a.(i) in
+    let t2 = bval bLen b i in
+    (if not (eq_u64 t1 t2) then false else bn_is_equal_ a b i)
+  else true
+
+// This is straightforward copy of bn_is_less. There must be a better
+// way to compare buffers.
+val bn_is_equal:
+     #aLen:bn_len
+  -> #bLen:bn_len{v bLen <= v aLen}
+  -> a:lbignum aLen
+  -> b:lbignum bLen
+  -> Stack bool
+    (requires fun h -> live h a /\ live h b)
+    (ensures  fun h0 r h1 -> modifies loc_none h0 h1 /\ h0 == h1 /\ r == (as_snat h0 a = as_snat h0 b))
+let bn_is_equal #aLen #bLen a b = admit(); bn_is_equal_ a b aLen
